protocols/NeedhamSchroeder.v
@@ -260,9 +260,61 @@ Module MyProtocolSecure <: AutomatedSafeProtocol.
       gen1.
       gen1.
       gen1.
+
+      eapply msc_step_alt.
+      + unfold oneStepClosure_new; repeat gen1'.
+
+        match goal with
+        | [ S : step ?st _ |- _ ] =>
+          concrete st;
+            match goal with
+            | [ LA : labels_align ?st |- _ ] =>
+              eapply label_align_step_split in S; (reflexivity || eauto 2)
+            | _ =>
+              assert (labels_align st) (* by ((repeat prove_alignment1); eauto) *)
+            end
+        end.
+
+        
+
       gen1.
       gen1.
       gen1.
+
+      eapply msc_step_alt.
+      unfold oneStepClosure_new; repeat gen1'.
+
+      simplify
+    ; tidy
+    ; rstep
+    ; istep
+    ; subst
+    ; canonicalize users
+    ; repeat close
+      
+      ; [ solve[ unfold oneStepClosure_new; repeat gen1' ]
+        | solve[ simplify
+                 ; sets
+                 ; split_ex
+                 ; propositional
+                 ; repeat match goal with
+                          | [H : (?x1, ?y1) = ?p |- _] =>
+                            match p with
+                            | (?x2, ?y2) =>
+                              tryif (concrete x2; concrete y2)
+                              then let H' := fresh H
+                                   in assert (H' : (x1, y1) = (x2, y2) -> x1 = x2 /\ y1 = y2)
+                                     by equality
+                                      ; propositional
+                                      ; discriminate
+                              else invert H
+                            | _ => invert H
+                            end
+                          end
+               | eapply intersect_empty_l]
+        | rewrite ?union_empty_r ]
+
+
       
     (* The remaining parts of the proof script shouldn't need to change. *)
     - intros.
